Fix pad_message and prove cheat

examples/Crypto/SHA-2/sha2Script.sml
@@ -1,7 +1,7 @@
 open HolKernel boolLib bossLib Parse
-     listTheory rich_listTheory arithmeticTheory
-     wordsTheory numposrepTheory byteTheory wordsLib
-     cv_transLib cv_stdTheory
+     listTheory rich_listTheory arithmeticTheory logrootTheory
+     bitTheory wordsTheory numposrepTheory byteTheory wordsLib
+     dividesTheory cv_transLib cv_stdTheory
 
 (* The SHA-2 Standard: https://nvlpubs.nist.gov/nistpubs/FIPS/NIST.FIPS.180-4.pdf *)
 (* SHA-256 in particular (i.e. Section 6.2) *)
@@ -21,7 +21,7 @@ val () = cv_auto_trans numposrepTheory.n2l_n2lA;
 Definition pad_message_def:
   pad_message bs =
   let l = LENGTH bs in
-  let n = l + 1 MOD 512 in
+  let n = (l + 1) MOD 512 in
   let k = if n <= 448 then 448 - n else 512 + 448 - n in
   let lb = PAD_LEFT 0 64 $ (if l = 0 then [] else REVERSE $ n2l 2 l) in
   let bits = MAP bool_to_bit bs in
@@ -34,8 +34,27 @@ Theorem pad_message_length_multiple:
   LENGTH bs < 2 ** 64 ==>
   divides 512 $ LENGTH (pad_message bs)
 Proof
-  rw[pad_message_def, PAD_LEFT, LENGTH_n2l, ADD1]
-  \\ cheat
+  rewrite_tac[pad_message_def, PAD_LEFT, ADD1]
+  \\ strip_tac
+  \\ BasicProvers.LET_ELIM_TAC
+  \\ rw[Abbr`bits`]
+  \\ Cases_on`l = 0` \\ gs[Abbr`n`, Abbr`lb`, Abbr`k`]
+  \\ simp[LENGTH_n2l, ADD1, LOG2_def]
+  \\ `LOG2 l < 64`
+  by ( qspecl_then[`l`,`64`]mp_tac LT_TWOEXP \\ simp[] )
+  \\ gs[LOG2_def]
+  \\ qspec_then `512` mp_tac DIVISION
+  \\ impl_tac >- rw[]
+  \\ disch_then(qspec_then`l + 1`mp_tac)
+  \\ strip_tac
+  \\ qpat_x_assum`l + 1 = _`(assume_tac o SYM)
+  \\ `(l + 1) MOD 512 = l + 1 - (l + 1) DIV 512 * 512` by simp[]
+  \\ pop_assum SUBST1_TAC
+  \\ IF_CASES_TAC
+  \\ simp[]
+  \\ irule DIVIDES_ADD_1
+  \\ simp[]
+  \\ simp[divides_def]
 QED
 
 Definition parse_block_def:
